cfrontend/SimplExpr.v
@@ -654,4 +654,5 @@ Definition transl_program (p: Csyntax.program) : res program :=
         prog_comp_env_eq := prog_comp_env_eq p;
         prog_pol_pub := AST.prog_pol_pub p1;
         prog_agr_comps := AST.prog_agr_comps p1;
+        prog_pol_complete := AST.prog_pol_complete p1;
      |}.
